Nonogram.lean
@@ -1,3 +1,4 @@
 import Nonogram.Rule
 import Nonogram.LineSolver.Soundness
+import Nonogram.LineSolver.Board.Soundness
 import Nonogram.Tactic
